extract_to_expand_inequality

lean3/src/bound.lean
@@ -1,6 +1,7 @@
 import testbed.graph_theory
 import get_theorems
 import get_subexpressions
+import change_hypothesis
 
 open simple_graph 
 open expr tactic
@@ -68,9 +69,9 @@ meta def get_lower_bounds_on (e : expr) : tactic (list name) := do {
 #eval (to_expr ``((@finset.univ _ _).card)) >>= get_lower_bounds_on >>= trace -- [degree_bound ]
 
 
---------------------  TACTIC: EXPAND INEQUALITY A ≤ C to A ≤ B and B ≤ C -------------------- 
+--------------------  TACTIC: IF GOAL IS A ≤ C, EXTRACT STATEMENTS OF FORM A ≤ B and B ≤ C -------------------- 
 
-meta def expand_inequality : tactic unit :=
+meta def extract_to_expand_inequality : tactic unit :=
 do {
   `(%%lhs ≤ %%rhs) ← target,
 
@@ -83,36 +84,24 @@ do {
   -- make sure everything is in the numerator (so expr2 really is an upper bound when you have expr1 ≤ expr2)
 
   -- loop thorugh all naturals in left side (call them le)
-  -- and all naturals in right side (call them re)
-  -- and try to find if the library has an expression of form  _(le)_ ≤_(B)_ and another of form _(B)_ ≤ _(re)_ 
-  -- where the notation _(x)_ means "an expression involving x"
+  -- and add statements that give upper bounds on them to the hypothesis
   lexp.mmap $ λle, do { 
-    -- get all upper bounds on the lefthand side
-
-    -- statement ← get_thm_statement `degree_sum, 
-
-    -- statement ← without_quantifiers statement, 
-   -- torf ← contains_subexpr statement le ,
-
-    -- torf ← is_upper_bound_on statement le,
-    -- trace torf,
-    -- skip
-    -- trace torf
     upper_bounds ← get_upper_bounds_on le,
-    trace upper_bounds,
-    skip
-    -- upper_bounds.mmap $ λ n, do {
-    --   add_theorem_to_hypothesis n
-    -- }
+    upper_bounds.mmap $ λ n, do {
+      in_hyp ← in_hypothesis n,
+      if in_hyp then skip else add_theorem_to_hypothesis n
+    }
   },
 
-  -- rexp.mmap $ λre, do {
-  --   trace le,
-  --   with_le ← get_upper_bounds_on le,
-  --   trace with_le,
-  --   trace "",
-  --   skip
-  -- },
+ -- loop thorugh all naturals in right side (call them re)
+  -- and add statements that give lower bounds on them to the hypothesis
+  rexp.mmap $ λre, do {
+    lower_bounds ← get_lower_bounds_on re,
+    lower_bounds.mmap $ λ n, do {
+      in_hyp ← in_hypothesis n,
+      if in_hyp then skip else add_theorem_to_hypothesis n
+    }
+  },
 
   -- alternative to make things more efficient:
   -- loop thorugh all naturals in left side (call them le)
@@ -132,11 +121,16 @@ do {
   skip
 }
 
+--------------------  TACTIC: EXPAND INEQUALITY A ≤ C to A ≤ B and B ≤ C -------------------- 
+
+
+
 -- variables {G : simple_graph V} [fintype V] [decidable_rel G.adj] [decidable_eq V]
 
 -- Graphs have at most (n choose 2) edges (the automated version) --
 theorem edge_bound_auto (G : simple_graph V) [fintype V] [decidable_rel G.adj] [decidable_eq V]: 
   ∣∣E[G]∣∣ ≤ ∣∣(V[G])∣∣.choose 2 :=
 begin 
-  expand_inequality,
+  extract_to_expand_inequality,
+  -- expand_inequality
 end
